pulse/examples/steel/LineStruct.fst
@@ -61,40 +61,22 @@ let merge_line p1 p2 p1' p2'
 
 /// Taking pointers to the p1 and p2 fields of a line
 
-let addr_of_p1 (#p1 #p2: Ghost.erased point) (p: ref 'a line{p.q == line_pcm})
-: SteelT (q:ref 'a point{q == ref_focus p point_pcm _p1})
-    (p `pts_to` mk_line p1 p2)
-    (fun q ->
-       (p `pts_to` mk_line (one point_pcm) p2) `star`
-       (q `pts_to` p1))
-= let q = addr_of_lens p _p1 (mk_line p1 p2) in
+let addr_of_p1 #a #p1 #p2 p =
+  let q = addr_of_lens p _p1 (mk_line p1 p2) in
   A.change_equal_slprop (p `pts_to` _) (p `pts_to` mk_line (one point_pcm) p2);
   A.change_equal_slprop (q `pts_to` _) (q `pts_to` p1);
   A.return q
 
-let un_addr_of_p1 (#p1 #p2: Ghost.erased point)
-  (p: ref 'a line{p.q == line_pcm}) (q: ref 'a point{q == ref_focus p point_pcm _p1})
-: SteelT unit
-    ((p `pts_to` mk_line (one point_pcm) p2) `star` (q `pts_to` p1))
-    (fun q -> p `pts_to` mk_line p1 p2)
-= un_addr_of_lens q p _p1 (mk_line (one point_pcm) p2) p1;
+let un_addr_of_p1 #a #p1 #p2 p q =
+  un_addr_of_lens q p _p1 (mk_line (one point_pcm) p2) p1;
   A.change_equal_slprop (p `pts_to` _) (p `pts_to` _)
 
-let addr_of_p2 (#p1 #p2: Ghost.erased point) (p: ref 'a line{p.q == line_pcm})
-: SteelT (q:ref 'a point{q == ref_focus p point_pcm _p2})
-    (p `pts_to` mk_line p1 p2)
-    (fun q ->
-       (p `pts_to` mk_line p1 (one point_pcm)) `star`
-       (q `pts_to` p2))
-= let q = addr_of_lens p _p2 (mk_line p1 p2) in
+let addr_of_p2 #a #p1 #p2 p =
+  let q = addr_of_lens p _p2 (mk_line p1 p2) in
   A.change_equal_slprop (p `pts_to` _) (p `pts_to` mk_line p1 (one point_pcm));
   A.change_equal_slprop (q `pts_to` _) (q `pts_to` p2);
   A.return q
 
-let un_addr_of_p2 (#p1 #p2: Ghost.erased point)
-  (p: ref 'a line{p.q == line_pcm}) (q: ref 'a point{q == ref_focus p point_pcm _p2})
-: SteelT unit
-    ((p `pts_to` mk_line p1 (one point_pcm)) `star` (q `pts_to` p2))
-    (fun q -> p `pts_to` mk_line p1 p2)
-= un_addr_of_lens q p _p2 (mk_line p1 (one point_pcm)) p2;
+let un_addr_of_p2 #a #p1 #p2 p q =
+  un_addr_of_lens q p _p2 (mk_line p1 (one point_pcm)) p2;
   A.change_equal_slprop (p `pts_to` _) (p `pts_to` _)
